updates

IrisProjects/InsertionSort.v
@@ -14,29 +14,36 @@ l2: None or l3
 l3: Sub-list [y, l3]
 
 ref ("i", ref ())
+ *)
+
+(*
+match: "l2" with
+   NONE => (if: ("x" ≤ "i")%E then "p" <- SOME ("x", ref ( SOME ("i", NONE)) ) else "p" <- SOME ("i", ref (SOME ("x", NONE))) )
+   | SOME "l3" => 
+    let: "y" := Fst !"l3" in  (* Second element *)
+    (if: (("x" ≤ "i")%E  && ("i" ≤ "y"))%E then "p" <- SOME("x", ref(SOME("i", ref(SOME("y", NONE)))))
+    else "p" <- SOME ("x",  "insert" "i" "l"))
+   end
 *)
+
+(* list A := option (ref (A * list A)) *)
 
 (* insert i into its sorted place in list l *)
 Definition insert : val := 
  rec: "insert" "i" "l" := 
   match: "l" with           (* A list is either... *)
-  NONE => ref (SOME( "i", NONE) )             (* ... the empty list *)
+  NONE => SOME( ref( "i", NONE))             (* ... the empty list *)
   | SOME "p" => 
    let: "x" := Fst !"p" in  (* First element - !e means  Load e%E *)
    let: "l2" := Snd !"p" in  (* Rest of the list *)
-   match: "l2" with
-   NONE => (if: ("x" ≤ "i")%E then "p" <- ref (SOME ("x", ref ( SOME ("i", NONE)) )) else "p" <- ref (SOME ("i", ref (SOME ("x", NONE)))) )
-   | SOME "l3" => 
-    let: "y" := Fst !"l3" in  (* Second element *)
-    (if: (("x" ≤ "i")%E  && ("i" ≤ "y"))%E then "p" <- ("x",  ("i"  "l") )
-    else "p" <- ("x",  "insert" "i" "l"))
-   end 
+   (if: ("i" ≤ "x")%E then  SOME(ref("i", "l"))
+   else SOME(ref("x", "insert" "i" "l2")))
   end.
 
 Definition sort : val := 
  rec: "sort" "l" := 
   match: "l" with 
-  NONE => #()
+  NONE => NONE
   | SOME "p" =>
   let: "x" := Fst !"p" in 
   let: "l" := Snd !"p" in 
@@ -92,7 +99,7 @@ Fixpoint sort_spec (l : list Z) (v : val) : iProp Σ :=
 Fixpoint insert_func (i : Z) (l : list Z) :=
   match l with
   | []  => [i]
-  | h :: t  => if (i <=? h)%Z then i :: h :: t else h :: insert_func i t
+  | h :: t  => if bool_decide (i <= h)%Z then i :: h :: t else h :: insert_func i t
   end.  
 
 
@@ -102,60 +109,89 @@ Fixpoint insert_func (i : Z) (l : list Z) :=
     (nth i l 0) ≤ (nth j l 0). *)
 
 (* Coq-level definition of Sorted from standard library modified to support integers Z *)
-Variable R : Z -> Z -> Prop.
 
-Inductive HdRel a : list Z -> Prop :=
-    | HdRel_nil : HdRel a []
-    | HdRel_cons b l : R a b -> HdRel a (b :: l).
+Check Sorted.
 
-Inductive Sorted : list Z -> Prop :=
-    | Sorted_nil : Sorted []
-    | Sorted_cons a l : Sorted l -> HdRel a l -> Sorted (a :: l).
+About Sorted. 
 
 (* list l is sorted. Insert i into the sorted list *)
 
 Lemma insertTest l:
   {{{⌜ l = NONE ⌝}}}
   insert #2 NONE 
-  {{{v',RET v'; is_list [2] v'}}}.
+  {{{v',RET v'; is_list  [2]  v'  }}}.
 Proof.
    iIntros (Φ) "Hl Post".
    unfold insert.
    wp_pures.
 
    wp_alloc g as "H".
-   iModIntro.
+   wp_pures. 
+   iModIntro. 
    iApply "Post".
-   unfold is_list.
-   iExists g.
-   iSplitR "H".
-   - iPureIntro. reflexivity.          
+   simpl.
+   iDestruct "Hl" as %->. 
+   iExists _. 
+   iSplit.
+   - iPureIntro. reflexivity.
+   - iExists NONEV. iFrame. iPureIntro.  reflexivity.
+   Qed. 
 
-
-  Admitted. 
+Lemma insert_func_hdrel : forall (i x : Z) (l : list Z),
+  HdRel Z.le x (insert_func i l).
+Proof.
+  intros i x l.
+  (* Induction on l *)
+  induction l as [| y l' IHl].
+  - (* Base case: l = [] *)
+    simpl.
+    admit. 
+    (* Prove the base case *)
+    (* You may need additional lemmas or properties here *)
+    (* It might involve proving that x is less than or equal to the inserted element *)
+  - (* Inductive case: l = y :: l' *)
+    simpl.
+    admit. 
+    (* Prove the inductive step *)
+    (* Use properties of insert_func, HdRel, and Z.le here *)
+    (* You may need to use transitivity of Z.le *)
+Admitted.
 
 Lemma insert_proof l v (i:Z): 
-  {{{is_list l v}}}
+  {{{ ⌜Sorted (≤) l⌝ ∗  is_list l v }}}
   insert #i v
-  {{{v',RET v'; is_list (insert_func i l) v' ∗ ⌜ Sorted (insert_func i l) ⌝}}}.  
+  {{{v',RET v'; is_list (insert_func i l) v' ∗ ⌜ Sorted (≤) (insert_func i l) ⌝}}}.  
 Proof. 
   (* Proof *)
   iIntros (Φ) "Hl Post".
-  unfold insert.
-  wp_rec.
-  wp_let.
-  unfold insert_func.
-
+  iDestruct "Hl" as (Heq)  "Hl". 
   iInduction l as [|x l] "IH" forall (v Φ); simpl.
   - iDestruct "Hl" as %->.
-     wp_pures. 
-     wp_alloc l as "H".
-     iModIntro.  
-     iApply "Post".
-     iSplitL "H".
-     {iExists l.  }    
-  (* - iDestruct "Hl" as (p) "[-> Hl]". iDestruct "Hl" as (v) "[Hp Hl]".  *)
+    wp_rec. wp_let. wp_match.
+    wp_alloc g as "H".
+    wp_pures.
+    iModIntro. 
+    iApply "Post".
+    iSplitL "H".
+    {iExists g. iSplitR "H". {iPureIntro. reflexivity.} { iExists NONEV. iFrame. iPureIntro.  reflexivity.}}
+    {iPureIntro. apply Sorted_cons. {apply Sorted_nil.} { auto. } }
+  - iDestruct "Hl" as (p) "[-> Hl]". iDestruct "Hl" as (v) "[Hp Hl]".
+    wp_rec. wp_let. wp_match. wp_load. wp_proj.
+    wp_let. wp_load. wp_proj. wp_let.
+    wp_pure.  case_bool_decide. 
+    + wp_if_true. wp_alloc g as "list". wp_pures.
+      iModIntro.
+      iApply "Post".
+      iSplit.
+      { simpl. eauto 10 with iFrame. }
+      { iPureIntro. apply Sorted_cons. {exact.} {apply HdRel_cons. exact. } }
+    + wp_if_false.  wp_apply ("IH" with" [] [$Hl]").
+      { iPureIntro. admit.  }
+      { iIntros (v') "[islist %HS]". wp_alloc g as "list". wp_pures. iModIntro. iApply "Post". iSplit. { simpl. eauto 10 with iFrame.} {iPureIntro. apply Sorted_cons. { exact.
+} {simpl. apply insert_func_hdrel.} }  }
+
 Admitted. 
+
 
 
 Lemma sort_proof l v:
